wip

src/db/injection.lean
@@ -5,23 +5,108 @@ This file contains the injection of `db` into `exp`.
 -/
 
 import .type
-import exp
+import aeq
 
 namespace acie -----------------------------------------------------------------
 namespace db -------------------------------------------------------------------
 
 variables {V : Type} [decidable_eq V] -- Type of variable names
 variables {vs : Type → Type} [vset vs V] -- Type of variable name sets
-variables {X : vs V} -- Variable name sets
+variables {X Y : vs V} -- Variable name sets
 variables {n : ℕ} -- De Bruijn indexes
 
-def inject_lam (a : V) (ϕ : ν∈ X → fin n) (x : ν∈ (insert a X)) : fin (nat.succ n) :=
+def inject.lam (a : V) (ϕ : ν∈ X → fin n) (x : ν∈ (insert a X)) : fin (nat.succ n) :=
   if p : x.1 = a then fin.of_nat 0 else fin.succ $ ϕ $ vname.erase x p
 
 def inject : ∀ {X : vs V}, exp X → ∀ {n : ℕ}, (ν∈ X → fin n) → db n
   | X (exp.var x)              n ϕ := db.var $ ϕ x
   | X (exp.app f e)            n ϕ := db.app (inject f ϕ) (inject e ϕ)
-  | X (@exp.lam _ _ _ _ _ a e) n ϕ := db.lam $ inject e $ inject_lam a ϕ
+  | X (@exp.lam _ _ _ _ _ a e) n ϕ := db.lam $ inject e $ acie.db.inject.lam a ϕ
+
+def blah (ϕ₁ : ν∈ X → fin n) (ϕ₂ : ν∈ Y → fin n) : X ×ν Y:=
+  λ (x : ν∈ X) (y : ν∈ Y), ϕ₁ x = ϕ₂ y
+
+theorem inj_blah (ϕ₁ : ν∈ X → fin n) (ϕ₂ : ν∈ Y → fin n) (e₁ : exp X) (e₂ : exp Y)
+: (e₁ ≡α⟨blah ϕ₁ ϕ₂⟩ e₂) ↔ (inject e₁ ϕ₁ = inject e₂ ϕ₂) :=
+  begin
+    induction e₁ with
+      /- var -/ X x
+      /- app -/ X f₁ e₁ rf re
+      /- lam -/ X a e₁ r
+      generalizing Y ϕ₁ ϕ₂ e₂,
+    begin /- var -/
+      cases e₂ with
+        /- var -/ Y y
+        /- app -/ Y f₂ e₂
+        /- lam -/ Y b e₂,
+      begin /- var -/
+        simp [inject],
+        split,
+        begin /- iff.mp -/
+          intro α,
+          have h : ϕ₁ x = ϕ₂ y, from aeq.var.prop α,
+          rw [h]
+        end,
+        begin /- iff.mpr -/
+          intro p,
+          have h : ϕ₁ x = ϕ₂ y, from db.var.inj p,
+          exact aeq.var h
+        end
+      end,
+      begin /- app -/
+        split, repeat { intro x, cases x }
+      end,
+      begin /- lam -/
+        split, repeat { intro x, cases x }
+      end
+    end,
+    begin /- app -/
+      cases e₂ with
+        /- var -/ Y y
+        /- app -/ Y f₂ e₂
+        /- lam -/ Y b e₂,
+      begin /- var -/
+        split, repeat { intro x, cases x },
+      end,
+      begin /- app -/
+        simp [inject],
+        split,
+        begin /- iff.mp -/
+          intro α,
+          have αf : f₁ ≡α⟨blah ϕ₁ ϕ₂⟩ f₂, from aeq.app.fun α,
+          have αe : e₁ ≡α⟨blah ϕ₁ ϕ₂⟩ e₂, from aeq.app.arg α,
+          have pf : inject f₁ ϕ₁ = inject f₂ ϕ₂, from iff.mp (rf ϕ₁ ϕ₂ f₂) αf,
+          have pe : inject e₁ ϕ₁ = inject e₂ ϕ₂, from iff.mp (re ϕ₁ ϕ₂ e₂) αe,
+          rw [pf, pe]
+        end,
+        begin /- iff.mpr -/
+          intro p,
+          have h : inject f₁ ϕ₁ = inject f₂ ϕ₂ ∧ inject e₁ ϕ₁ = inject e₂ ϕ₂, from
+            db.app.inj p,
+          have αf : f₁ ≡α⟨blah ϕ₁ ϕ₂⟩ f₂, from iff.mpr (rf ϕ₁ ϕ₂ f₂) h.1,
+          have αe : e₁ ≡α⟨blah ϕ₁ ϕ₂⟩ e₂, from iff.mpr (re ϕ₁ ϕ₂ e₂) h.2,
+          exact aeq.app αf αe
+        end
+      end,
+      begin /- lam -/
+        split, repeat { intro x, cases x },
+      end
+    end,
+    begin /- lam -/
+      cases e₂ with
+        /- var -/ Y y
+        /- app -/ Y f₂ e₂
+        /- lam -/ Y b e₂,
+      begin /- var -/
+        split, repeat { intro x, cases x },
+      end,
+      begin /- app -/
+        split, repeat { intro x, cases x },
+      end,
+      begin /- lam -/
+      end
+    end
+  end
 
 end /- namespace -/ db ---------------------------------------------------------
 end /- namespace -/ acie -------------------------------------------------------
